Modified Disquotation: started implementing translation lt -> lpa.

FormalizingAxiomaticTheoriesOfTruth/Disquotation.lean
@@ -6,11 +6,88 @@ open FirstOrder
 /-
 # The definition of TB
 -/
-namespace TB
 open L_T
 open PAT
+namespace TB
 def disquotation_schema (φ : Semiformula lt ℕ 0) : SyntacticFormula lt :=
   .rel .t ![numeral (Semiformula.toNat (φ))] pt_bi_imp φ
 def disquotation_set (Γ : Semiformula lt ℕ 0 → Prop) : Theory lt :=
   { ψ | ∃ φ : Semiformula lt ℕ 0, Γ φ ∧ ψ = (disquotation_schema φ)}
 def tb : Theory lt := axiom_set + disquotation_set Set.univ
+
+end TB
+
+/-
+Proof that T⌜=(0,0)⌝ ↔ =(0,0) ∈ tb
+-/
+open L_T
+open TB
+def formula_eq_null : Semiformula lt ℕ 0 :=
+  .rel .eq ![null,null]
+def disquotation : Semiformula lt ℕ 0 :=
+  .rel .t ![numeral (formula_eq_null.toNat)] pt_bi_imp formula_eq_null
+example : disquotation ∈ tb := by
+  have step1 : (disquotation ∈ tb) = (disquotation ∈ axiom_set + {ψ | ∃ φ, Set.univ φ ∧ ψ = disquotation_schema φ}) := by
+    rw[tb,disquotation_set]
+  have step2 : formula_eq_null ∈ Set.univ := by simp
+  have step3 : Set.univ formula_eq_null := by
+    apply step2
+  have step4 : disquotation = disquotation_schema formula_eq_null := by
+    rw[disquotation_schema,disquotation]
+  have step5 : Set.univ formula_eq_null ∧ disquotation = disquotation_schema formula_eq_null := by
+    apply And.intro
+    exact step3
+    exact step4
+  have step6 : ∃ φ, Set.univ φ ∧ disquotation = disquotation_schema φ := by
+    apply Exists.intro formula_eq_null step5
+  have step7 : disquotation ∈ {ψ | ∃ φ, Set.univ φ ∧ ψ = disquotation_schema φ} := by
+    exact step6
+  have step8 : disquotation ∈ {ψ | ∃ φ, Set.univ φ ∧ ψ = disquotation_schema φ} → disquotation ∈ axiom_set + {ψ | ∃ φ, Set.univ φ ∧ ψ = disquotation_schema φ} := by
+    apply Set.mem_union_right
+  have step9 : disquotation ∈ axiom_set + {ψ | ∃ φ, Set.univ φ ∧ ψ = disquotation_schema φ} := by
+    apply step8 step7
+  have step10 : disquotation ∈ tb := by
+    apply step1.mpr step9
+  exact step10
+
+/-
+A function for translating PA.lpa formulas to L_T.lt formulas
+-/
+open PA
+def to_lt_func {arity : ℕ} : (lt.Func arity) → (lt.Func arity)
+  | .zero => .zero
+  | .succ => .succ
+  | .add => .add
+  | .mult => .mult
+
+def to_lt_rel {n : ℕ} : (lpa.Rel n) → (lt.Rel n)
+  | .eq => .eq
+
+def to_lt_t {n : ℕ}: Semiterm lpa ℕ n → Semiterm lt ℕ n
+  | #x => #x
+  | &x => &x
+  | .func f v => .func (to_lt_func f) (fun i => to_lt_t (v i))
+
+def to_lt_vt {k n: ℕ} (v : Fin k → Semiterm lpa ℕ n) : Fin k → Semiterm lt ℕ n :=
+  fun i => to_lt_t (v i)
+
+def to_lt_f {n : ℕ} : Semiformula lpa ℕ n → Semiformula lt ℕ n
+| .verum => .verum
+| .falsum => .falsum
+| .rel r v => .rel (to_lt_rel r) (to_lt_vt v)
+| .nrel r v => .nrel (to_lt_rel r) (to_lt_vt v)
+| .and φ ψ => .and (to_lt_f φ) (to_lt_f ψ)
+| .or φ ψ => .or (to_lt_f φ) (to_lt_f ψ)
+| .all φ => .all (to_lt_f φ)
+| .ex φ => .ex (to_lt_f φ)
+
+example {n : ℕ}: ∀φ:Semiformula lpa ℕ n, ∃ψ:Semiformula lt ℕ n, ψ = to_lt_f φ :=
+  fun a : Semiformula lpa ℕ n => Exists.intro (to_lt_f a) (Eq.refl (to_lt_f a))
+
+/-
+Function for translating derivations from tb to derivations from t_pa
+-/
+open TB
+-- def to_pa_der {n : ℕ} (φ : Semiformula lt ℕ 0) (ψ : Semiformula lpa ℕ 0) (h : φ = to_lt_f ψ): Derivation tb (φ :: Γ) → Derivation t_pa (ψ :: Δ)
+-- | .root φ => .root ψ
+-- | .axL (φ :: Γ) r v => .axL (ψ :: Δ) r v
